STLC_SuccNat/Lifted_Norm.v
@@ -133,7 +133,7 @@ Proof.
   split. apply (step'_preserves_halting _ _ E); eauto.
   intros.
   eapply IHT'2.
-  apply  ST_App1'. apply E.
+  apply  ST_App'. apply E.
   apply RRt; auto.
   (* Nat *)
   split. eapply preservation'; eauto.
@@ -161,7 +161,7 @@ Proof.
   eapply IHT'2.
   eapply T_App'; eauto.
   apply R'_typable_empty; auto.
-  eapply ST_App1'. apply E.
+  eapply ST_App'. apply E.
   apply RRt; auto.
   (* Nat *)
   split. auto.
@@ -289,10 +289,10 @@ Qed.
 
 Inductive instantiation' : tass' -> env' -> Prop :=
   | V_nil' : instantiation' nil nil
-  | V_cons' : forall x T' v' c e,
-      value' v' -> R' T' v' ->
+  | V_cons' : forall x T' t' c e,
+      R' T' t' ->
       instantiation' c e ->
-      instantiation' ((x,T')::c) ((x,v')::e).
+      instantiation' ((x,T')::c) ((x,t')::e).
 
 Lemma instantiation'_domains_match: forall {c} {e},
   instantiation' c e ->
@@ -321,7 +321,7 @@ Lemma instantiation'_R' : forall c e,
     lookup x c = Some T' ->
     lookup x e = Some t' -> R' T' t'.
 Proof.
-  intros c e V. induction V; intros x' t' T1' G E.
+  intros c e V. induction V; intros x' t1' T1' G E.
     solve_by_inverts 1.
     unfold lookup in *. destruct (eqb x x').
       inversion G; inversion E; subst. auto.
@@ -360,10 +360,10 @@ Lemma msubst'_preserves_typing : forall c e,
 Proof.
     intros c e H. induction H; intros.
     simpl in H. simpl. auto.
-    simpl in H2.  simpl.
+    simpl in H1.  simpl.
     apply IHinstantiation'.
     eapply substitution_preserves_typing'; eauto.
-    apply (R'_typable_empty H0).
+    apply (R'_typable_empty H).
 Qed.
 
 Lemma msubst'_R' : forall c env' t' T',
@@ -402,21 +402,19 @@ Proof.
         unfold R'. fold R'. split.
            auto.
          split. apply value'_halts'. apply v_abs'.
-         intros.
-         destruct (R'_halts' H0) as [v [P Q] ].
-         pose proof (multistep'_preserves_R' _ _ _ P H0).
-         apply multistep'_preserves_R1' with (msubst' ((x,v)::env0') t').
+         intros. specialize IHHT with (c:=((x,T2')::c)).
+         assert (forall x0 : string, (x) |-> T2'; Gamma' x0 = lookup x0 ((x, T2') :: c)).
+         { intros. unfold update, t_update, lookup. destruct (String.eqb x x0); auto. }
+         eapply IHHT in H1.
+         apply multistep'_preserves_R1' with (msubst' ((x,s')::env0') t').
             eapply T_App'. eauto.
             apply R'_typable_empty; auto.
-            eapply multi_step'_trans. eapply multistep'_App2'; eauto.
-            eapply multi_step with (y:= (msubst' ((x, v) :: env0') t')); [|apply multi_refl].
-            simpl.  rewrite subst'_msubst'.
-            eapply ST_AppAbs'; eauto.
+            eapply multi_step. apply ST_AppAbs'.
+            simpl.  rewrite subst'_msubst'. apply multi_refl.
             eapply typable_empty__closed'.
-            apply (R'_typable_empty H1).
+            apply (R'_typable_empty H0).
             eapply instantiation'_env'_closed'; eauto.
-            eapply (IHHT ((x,T2')::c)).
-               intros. unfold update, t_update, lookup. destruct (String.eqb x x0); auto.
+            eassumption.
             constructor; auto.
   - (* T_App' *)
     rewrite msubst'_app'.
